```latex
\section*{Example 2}

Consider the differential equation:
\begin{equation}
    u_x + y u_y = 0.
\end{equation}

Let \( y' = - \frac{u_x}{u_y} = y \). Then, the solution can be expressed as:
\begin{equation}
    y = ce^{x},
\end{equation}
where \( c \) is a constant. Thus, we have:
\begin{equation}
    u(x, y) = u(0, ce^{x}) = F(ce^{x}).
\end{equation}

\section*{Example ?}

In the previous example, if in addition \( u(0, y) = 3 \), then what is the solution?

\subsection*{Solution}

Given \( u(0, y) = 3 \), we have:
\begin{equation}
    u(x, y) = F(ye^{x}) = u(0, y) = 3.
\end{equation}
Thus, the solution is:
\begin{equation}
    u(x, y) = 3.
\end{equation}
```
