```latex
\section*{Equations and Transformations}

\begin{align}
    4(x) &= (x + 0) = c f(x) - 38'(x) \\
    \int (y(x)) \, dx &= f(x) - g(x) \\
    f + y &= 4 \\
    f - g &= \int 4(x) \, dx \\
    f &= k + \int t(y(x)) \, dx \\
    g &= d - \int t(4(x)) \, dx
\end{align}

\subsection*{Rewrite}

\begin{align}
    f(x) &= za(x) + So \\
    g(x) &= 1P(x) - E
\end{align}

\subsection*{Function Transformation}

\begin{align}
    u(x +) &= f(x + H) + g(x - t) \\
    &= \left( d(x + t) + q(x - Ct) \right) + y(s) \, ds
\end{align}

\subsection*{d'Alembert Formula}

\begin{equation}
    \int \left( d(x + t) + q(x - Ct) \right) + y(s) \, ds
\end{equation}
```
