```latex
\section*{Equations and Solutions}

\begin{align}
    U_g &= U_{se} + U_s = c(U_{ss} - U_{su}) \\
    U_n &= U_g + U_{ng} = c(U_{gy} - U_{nn}) \\
    U_H &= 2(U_{es} + U_{ng}) - 2cU_{gy} \\
    U_x &= 4 + Y_y \\
    U_{xx} &= U_{gg} + U_{ny} + 213
\end{align}

\begin{equation}
    0 = U_H - in_x = -45U_{gy}
\end{equation}

\begin{equation}
    \text{KeyO: } \Theta U_g() = \text{fixtc} + \text{gla}
\end{equation}

\begin{equation}
    U_H - cU_{xx} = 0
\end{equation}

\begin{equation}
    u(x, 0) = f(x)
\end{equation}

\begin{equation}
    u_f(x, 0) = 4(X)
\end{equation}

\section*{Solution}

\begin{equation}
    u(x, t) = f(x + t) + g(x - ct)
\end{equation}

Let \( t = 0 \), then

\begin{equation}
    u(x, 0) = f(x) + f(x)
\end{equation}

\begin{equation}
    U^+(x, t) = cf'(x + t) - cg(x - t)
\end{equation}
```
