```latex
\section*{Implicit Differentiation}

Consider the equation:

\begin{equation}
1 + xy = 0.
\end{equation}

The function \( u(x, y) \) is not defined on the curve \( y = -y \).

In general, if \( a(x, y)(x + b(x, y))y = 0 \), the ordinary differential equation (ODE) is:

\begin{equation}
y = \ldots
\end{equation}

Assume \( y = Y(x) \) is implicitly defined by the equation \( U(x, y) = 0 \). Then:

\begin{equation}
u(x, y(x)) = 0.
\end{equation}

Differentiating implicitly, we have:

\begin{align}
u_x + y' u_y &= 0, \\
y' &= -\frac{u_x}{u_y}.
\end{align}

This is equivalent to:

\begin{equation}
S \cdot Nx + y = 0.
\end{equation}

\begin{equation}
y = \ldots
\end{equation}
```
