```latex
\section*{Chapter 2: Wave and Diffusion}

\subsection*{2.1 The Wave Equation}

Assume \( U = U(x, t) \) and \( U_{tt} = c^2 U_{xx} \) with \( c > 0 \).

\textbf{Theorem:} The general solutions of the wave equation are given by
\[
u(x, t) = f(x + ct) + g(x - ct),
\]
where \( f \) and \( g \) are arbitrary functions.

\textbf{Proof:}

Assume
\[
U_{tt} - c^2 U_{xx} = 0.
\]

Let \( V = U_t + c U_x \) and \( W = U_t - c U_x \). Then,
\[
V_t - c V_x = 0 \quad \text{and} \quad W_t + c W_x = 0.
\]

The solutions to these equations are
\[
v(x, t) = h(x + ct) \quad \text{and} \quad w(x, t) = k(x - ct),
\]
where \( h \) and \( k \) are arbitrary functions.

Thus, the general solution is
\[
u(x, t) = f(x + ct) + g(x - ct).
\]
```
