```latex
\section*{Example 2}

Consider the differential equation:

\begin{equation}
    u_x + y u_y = 0.
\end{equation}

We have the following conditions:

\begin{align}
    y' &= -y, \\
    y &= ce^{-x}, \\
    c &= y e^x, \\
    u(x, ce^{-x}) &= u(0, c) = u(0, y e^x) = F(y e^x).
\end{align}

\section*{Example ?}

In the previous example, if in addition \( u(0, y) = 3 \), then what is the solution?

\section*{Solution}

The solution is given by:

\begin{equation}
    u(x, y) = F(y e^x) = u(0, y) = F(y) = 3.
\end{equation}
```
