```latex
\section*{Wave Equation Solutions}

\subsection*{General Solution of the Homogeneous Equation}

Find the general solution of the homogeneous equation, which is given by:

\begin{equation}
    u_{tt} + c^2 u_{xx} = 0
\end{equation}

The solution can be expressed as:

\begin{equation}
    u = g(x - ct)
\end{equation}

\subsection*{Particular Solution}

Find a particular solution by assuming:

\begin{equation}
    u = f(x + ct)
\end{equation}

Then, we have:

\begin{align}
    u_t &= c f'(x + ct) \\
    u_x &= f'(x + ct)
\end{align}

Substituting into the wave equation:

\begin{equation}
    u_{tt} + c^2 u_{xx} = c^2 f''(x + ct) = h(x + ct)
\end{equation}

Thus, we find:

\begin{equation}
    f(x) = \int h(x) \, dx
\end{equation}

The general solution of the wave equation is:

\begin{equation}
    u = g(x - ct) + f(x + ct)
\end{equation}

\subsection*{Alternative Method: Change of Variables}

Alternatively, we can solve the equation by changing variables. Let:

\begin{align}
    \xi &= x + ct \\
    \eta &= x - ct
\end{align}

Then, the derivatives transform as follows:

\begin{align}
    u_t &= c u_\xi - c u_\eta \\
    u_x &= u_\xi + u_\eta
\end{align}

This transformation simplifies the wave equation to:

\begin{equation}
    u_{\xi \eta} = 0
\end{equation}

The solution in terms of the new variables is:

\begin{equation}
    u(\xi, \eta) = F(\xi) + G(\eta)
\end{equation}

where \( F \) and \( G \) are arbitrary functions determined by initial conditions.
```
